new/code/strings.v
@@ -99,8 +99,6 @@ Axiom repeatedTabs : ∀ {ext : ffi_syntax} {go_gctx : GoGlobalContext}, val.
 
 Definition asciiSpace {ext : ffi_syntax} {go_gctx : GoGlobalContext} : go_string := "strings.asciiSpace"%go.
 
-Axiom asciiSpace'init : ∀ {ext : ffi_syntax} {go_gctx : GoGlobalContext}, val.
-
 Definition Clone {ext : ffi_syntax} {go_gctx : GoGlobalContext} : go_string := "strings.Clone"%go.
 
 Definition Compare {ext : ffi_syntax} {go_gctx : GoGlobalContext} : go_string := "strings.Compare"%go.
@@ -261,7 +259,21 @@ Axiom _'init : ∀ {ext : ffi_syntax} {go_gctx : GoGlobalContext}, val.
 Definition initialize' {ext : ffi_syntax} {go_gctx : GoGlobalContext} : val :=
   λ: <>,
     package.init pkg_id.strings (λ: <>,
-      exception_do (do:  (asciiSpace'init #()))
+      exception_do (do:  (go.GlobalAlloc asciiSpace (go.ArrayType 256 go.uint8) #());;;
+      let: "$r0" := (let: "$k0" := #(W64 9) in
+      let: "$v1" := #(W8 1) in
+      let: "$k2" := #(W64 10) in
+      let: "$v3" := #(W8 1) in
+      let: "$k4" := #(W64 11) in
+      let: "$v5" := #(W8 1) in
+      let: "$k6" := #(W64 12) in
+      let: "$v7" := #(W8 1) in
+      let: "$k8" := #(W64 13) in
+      let: "$v9" := #(W8 1) in
+      let: "$k10" := #(W64 32) in
+      let: "$v11" := #(W8 1) in
+      CompositeLiteral (go.ArrayType 256 go.uint8) (LiteralValue [KeyedElement (Some (KeyExpression go.int "$k0")) (ElementExpression go.uint8 "$v1"); KeyedElement (Some (KeyExpression go.int "$k2")) (ElementExpression go.uint8 "$v3"); KeyedElement (Some (KeyExpression go.int "$k4")) (ElementExpression go.uint8 "$v5"); KeyedElement (Some (KeyExpression go.int "$k6")) (ElementExpression go.uint8 "$v7"); KeyedElement (Some (KeyExpression go.int "$k8")) (ElementExpression go.uint8 "$v9"); KeyedElement (Some (KeyExpression go.int "$k10")) (ElementExpression go.uint8 "$v11")])) in
+      do:  ((GlobalVarAddr asciiSpace #()) <-[go.ArrayType 256 go.uint8] "$r0"))
       ).
 
 Module Builder.
