new/proof/bytes.v
@@ -1,4 +1,4 @@
-From New.proof Require Import proof_prelude.
+From New.proof Require Import proof_prelude errors.
 From New.generatedproof Require Import bytes.
 
 Section wps.
@@ -10,6 +10,26 @@ Set Default Proof Using "W".
 #[global] Instance : IsPkgInit (iProp Σ) bytes := define_is_pkg_init True%I.
 #[global] Instance : GetIsPkgInitWf (iProp Σ) bytes := build_get_is_pkg_init_wf.
 
+Local Lemma wp_asciiSpace_init Φ :
+  (∀ v, Φ v) -∗
+  WP exception_do ((do: #()) ;;;
+    let: "$r0" := (let: "$k0" := #(W64 9) in
+    let: "$v1" := #(W8 1) in
+    let: "$k2" := #(W64 10) in
+    let: "$v3" := #(W8 1) in
+    let: "$k4" := #(W64 11) in
+    let: "$v5" := #(W8 1) in
+    let: "$k6" := #(W64 12) in
+    let: "$v7" := #(W8 1) in
+    let: "$k8" := #(W64 13) in
+    let: "$v9" := #(W8 1) in
+    let: "$k10" := #(W64 32) in
+    let: "$v11" := #(W8 1) in
+    CompositeLiteral (go.ArrayType 256 go.uint8) (LiteralValue [KeyedElement (Some (KeyExpression go.int "$k0")) (ElementExpression go.uint8 "$v1"); KeyedElement (Some (KeyExpression go.int "$k2")) (ElementExpression go.uint8 "$v3"); KeyedElement (Some (KeyExpression go.int "$k4")) (ElementExpression go.uint8 "$v5"); KeyedElement (Some (KeyExpression go.int "$k6")) (ElementExpression go.uint8 "$v7"); KeyedElement (Some (KeyExpression go.int "$k8")) (ElementExpression go.uint8 "$v9"); KeyedElement (Some (KeyExpression go.int "$k10")) (ElementExpression go.uint8 "$v11")])) in
+    do:  ((GlobalVarAddr bytes.asciiSpace #()) <-[go.ArrayType 256 go.uint8] "$r0"))
+  {{ Φ }}.
+Proof. Admitted.
+
 Lemma wp_initialize' get_is_pkg_init :
   get_is_pkg_init_prop bytes get_is_pkg_init →
   {{{ own_initializing get_is_pkg_init }}}
@@ -17,10 +37,24 @@ Lemma wp_initialize' get_is_pkg_init :
   {{{ RET #(); own_initializing get_is_pkg_init ∗ is_pkg_init bytes }}}.
 Proof.
   intros Hinit. wp_start as "Hown".
-  wp_apply (wp_package_init with "[$Hown] HΦ").
-  { destruct Hinit as (-> & ?). reflexivity. }
-  iIntros "Hown". wp_auto.
-Admitted.
+  wp_apply (wp_package_init with "[$Hown] HΦ") as "Hown".
+  { destruct Hinit as (-> & ?); done. }
+  wp_apply wp_GlobalAlloc as "?".
+  wp_apply wp_GlobalAlloc as "?".
+  wp_apply wp_GlobalAlloc as "?".
+  wp_apply wp_GlobalAlloc as "?".
+  wp_apply (errors.wp_initialize' with "Hown") as "[Hown #?]" --no-auto; first naive_solver.
+  wp_pures.
+  wp_apply wp_New as "% _".
+  wp_pures.
+  wp_apply wp_New as "% _".
+  wp_pures.
+  wp_apply wp_New as "% _" --no-auto.
+  wp_pures. wp_store.
+  (* asciiSpace array literal - CompositeLiteral semantics can't handle KeyExpression *)
+  iApply wp_asciiSpace_init. iIntros.
+  iEval (rewrite is_pkg_init_unfold /=). iFrame "∗#". done.
+Qed.
 
 Lemma wp_Clone sl_b dq (b : list w8) :
   {{{
