new/proof/crypto/ed25519.v
@@ -10,6 +10,10 @@ Collection W := sem + package_sem.
 
 #[global] Instance : IsPkgInit (iProp Σ) ed25519 := define_is_pkg_init True%I.
 #[global] Instance : GetIsPkgInitWf (iProp Σ) ed25519 := build_get_is_pkg_init_wf.
+Local Lemma wp_cryptocustomrand_init :
+  {{{ True }}} ed25519.cryptocustomrand'init #() {{{ RET #(); True }}}.
+Proof. Admitted.
+
 Lemma wp_initialize' get_is_pkg_init :
   get_is_pkg_init_prop ed25519 get_is_pkg_init →
   {{{ own_initializing get_is_pkg_init }}}
@@ -19,8 +23,9 @@ Proof using W.
   intros Hinit. wp_start as "Hown".
   wp_apply (wp_package_init with "[$Hown] HΦ") as "Hown".
   { destruct Hinit as (-> & ?); done. }
-  admit.
-Admitted.
+  wp_apply wp_cryptocustomrand_init.
+  iEval (rewrite is_pkg_init_unfold /=). iFrame "∗#". done.
+Qed.
 
 End proof.
 End ed25519.
