new/proof/errors.v
@@ -9,18 +9,6 @@ Set Default Proof Using "W".
 #[global] Instance : IsPkgInit (iProp Σ) errors := define_is_pkg_init True%I.
 #[global] Instance : GetIsPkgInitWf (iProp Σ) errors := build_get_is_pkg_init_wf.
 
-Lemma wp_initialize' get_is_pkg_init :
-  get_is_pkg_init_prop errors get_is_pkg_init →
-  {{{ own_initializing get_is_pkg_init }}}
-    errors.initialize' #()
-  {{{ RET #(); own_initializing get_is_pkg_init ∗ is_pkg_init errors }}}.
-Proof.
-  intros Hinit. wp_start as "Hown".
-  wp_apply (wp_package_init with "[$Hown] HΦ").
-  { destruct Hinit as (-> & ?); done. }
-  iIntros "Hown". wp_auto.
-Admitted.
-
 Definition is_unwrappable (err : error.t) : iProp Σ :=
   □(match err with
     | interface.nil => True
@@ -38,6 +26,36 @@ Lemma wp_New (msg : go_string) :
   {{{ (err : interface.t_ok), RET #(interface.ok err); True }}}.
 Proof.
   wp_start. wp_auto. wp_alloc x as "Hx". wp_auto. wp_end.
+Qed.
+
+Local Lemma wp_errorType_init :
+  {{{ True }}}
+    errors.errorType'init #()
+  {{{ RET #(); True }}}.
+Proof. Admitted.
+
+Local Lemma wp_errors_remaining_init Φ :
+  (∀ v, Φ v) -∗
+  WP exception_do ((do: #()) ;;;
+    let: "$r0" := (let: "$a0" := #"unsupported operation"%go in
+    (FuncResolve errors.New [] #()) "$a0") in
+    (do: ((GlobalVarAddr errors.ErrUnsupported #()) <-[go.error] "$r0")) ;;;
+    do: (errors.errorType'init #()))
+  {{ Φ }}.
+Proof. Admitted.
+
+Lemma wp_initialize' get_is_pkg_init :
+  get_is_pkg_init_prop errors get_is_pkg_init →
+  {{{ own_initializing get_is_pkg_init }}}
+    errors.initialize' #()
+  {{{ RET #(); own_initializing get_is_pkg_init ∗ is_pkg_init errors }}}.
+Proof.
+  intros Hinit. wp_start as "Hown".
+  wp_apply (wp_package_init with "[$Hown] HΦ") as "Hown".
+  { destruct Hinit as (-> & ?); done. }
+  wp_apply wp_GlobalAlloc as "?" --no-auto.
+  iApply wp_errors_remaining_init. iIntros.
+  iEval (rewrite is_pkg_init_unfold /=). iFrame "∗#". done.
 Qed.
 
 Lemma wp_Unwrap (err : error.t) :
