new/proof/fmt.v
@@ -1,5 +1,5 @@
 From New.generatedproof Require Import fmt.
-From New.proof Require Import io.
+From New.proof Require Import io errors.
 
 Section wps.
 Context `{hG: heapGS Σ, !ffi_semantics _ _}.
@@ -17,10 +17,14 @@ Lemma wp_initialize' get_is_pkg_init :
   {{{ RET #(); own_initializing get_is_pkg_init ∗ is_pkg_init fmt }}}.
 Proof.
   intros Hinit. wp_start as "Hown".
-  wp_apply (wp_package_init with "[$Hown] HΦ").
+  wp_apply (wp_package_init with "[$Hown] HΦ") as "Hown".
   { destruct Hinit as (-> & ?); done. }
-  iIntros "Hown". wp_auto.
-  iEval (rewrite is_pkg_init_unfold /=). iFrame "∗#".
+  do 5 (wp_apply wp_GlobalAlloc as "?").
+  wp_apply (io.wp_initialize' with "Hown") as "[Hown #?]" --no-auto; first naive_solver.
+  wp_pures.
+  wp_apply (errors.wp_initialize' with "Hown") as "[Hown #?]" --no-auto; first naive_solver.
+  (* remaining: ppFree/ssFree sync.Pool literals, space slice literal, errComplex/errBool errors.New *)
+  all: admit.
 Admitted.
 
 End wps.
