new/proof/io.v
@@ -10,13 +10,6 @@ Set Default Proof Using "W".
 #[global] Instance : IsPkgInit (iProp Σ) io := define_is_pkg_init True%I.
 #[global] Instance : GetIsPkgInitWf (iProp Σ) io := build_get_is_pkg_init_wf.
 
-Lemma wp_blackHolePool_init :
-  {{{ is_pkg_init sync }}}
-    io.blackHolePool'init #()
-  {{{ RET #(); True }}}.
-Proof.
-Admitted.
-
 Lemma wp_initialize' get_is_pkg_init :
   get_is_pkg_init_prop io get_is_pkg_init →
   {{{ own_initializing get_is_pkg_init }}}
@@ -24,16 +17,18 @@ Lemma wp_initialize' get_is_pkg_init :
   {{{ RET #(); own_initializing get_is_pkg_init ∗ is_pkg_init io }}}.
 Proof.
   intros Hinit. wp_start as "Hown".
-  wp_apply (wp_package_init with "[$Hown] HΦ").
+  wp_apply (wp_package_init with "[$Hown] HΦ") as "Hown".
   { destruct Hinit as (-> & ?); done. }
-  iIntros "Hown". wp_auto.
-  repeat wp_apply wp_GlobalAlloc as "?".
-  wp_apply (sync.wp_initialize' with "[$Hown]") as "(Hown & #?)"; first naive_solver.
-  wp_apply (errors.wp_initialize' with "[$Hown]") as "(Hown & #?)"; first naive_solver.
-  repeat wp_apply wp_New as "% _".
-  wp_apply wp_blackHolePool_init.
-  wp_apply wp_New as "% _".
-  iEval (rewrite is_pkg_init_unfold /=). iFrame "∗#". done.
-Qed.
+  do 11 (wp_apply wp_GlobalAlloc as "?").
+  wp_apply (sync.wp_initialize' with "Hown") as "[Hown #?]" --no-auto; first naive_solver.
+  wp_pures.
+  wp_apply (errors.wp_initialize' with "Hown") as "[Hown #?]" --no-auto; first naive_solver.
+  wp_pures.
+  do 7 (wp_apply wp_New as "% _"; wp_pures).
+  wp_apply wp_New as "% _" --no-auto.
+  wp_pures. wp_store.
+  (* remaining: Discard struct literal, blackHolePool sync.Pool literal, ErrClosedPipe errors.New *)
+  all: admit.
+Admitted.
 
 End wps.
