new/proof/log.v
@@ -1,6 +1,7 @@
 Require Import New.code.log.
 Require Import New.generatedproof.log.
 Require Import New.proof.proof_prelude.
+From New.proof Require Import sync io.
 
 Section wps.
 Context `{hG: heapGS Σ, !ffi_semantics _ _}.
@@ -8,8 +9,18 @@ Context {sem : go.Semantics} {package_sem : log.Assumptions}.
 Collection W := sem + package_sem.
 Set Default Proof Using "W".
 
+#[global] Instance : IsPkgInit (iProp Σ) os := define_is_pkg_init True%I.
+#[global] Instance : GetIsPkgInitWf (iProp Σ) os := build_get_is_pkg_init_wf.
+
 #[global] Instance : IsPkgInit (iProp Σ) log := define_is_pkg_init True%I.
 #[global] Instance : GetIsPkgInitWf (iProp Σ) log := build_get_is_pkg_init_wf.
+
+Local Lemma wp_os_initialize' get_is_pkg_init :
+  get_is_pkg_init_prop os get_is_pkg_init →
+  {{{ own_initializing get_is_pkg_init }}}
+    os.initialize' #()
+  {{{ RET #(); own_initializing get_is_pkg_init ∗ is_pkg_init os }}}.
+Proof. Admitted.
 
 Lemma wp_initialize' get_is_pkg_init :
   get_is_pkg_init_prop log get_is_pkg_init →
@@ -18,10 +29,16 @@ Lemma wp_initialize' get_is_pkg_init :
   {{{ RET #(); own_initializing get_is_pkg_init ∗ is_pkg_init log }}}.
 Proof.
   intros Hinit. wp_start as "Hown".
-  wp_apply (wp_package_init with "[$Hown] HΦ").
+  wp_apply (wp_package_init with "[$Hown] HΦ") as "Hown".
   { destruct Hinit as (-> & ?); done. }
-  iIntros "Hown". wp_auto.
-  iEval (rewrite is_pkg_init_unfold /=). iFrame "∗#".
+  do 2 (wp_apply wp_GlobalAlloc as "?").
+  wp_apply (sync.wp_initialize' with "Hown") as "[Hown #?]" --no-auto; first naive_solver.
+  wp_pures.
+  wp_apply (wp_os_initialize' with "Hown") as "[Hown #?]" --no-auto; first naive_solver.
+  wp_pures.
+  wp_apply (io.wp_initialize' with "Hown") as "[Hown #?]" --no-auto; first naive_solver.
+  (* remaining: log.New call for std logger, bufferPool sync.Pool literal *)
+  all: admit.
 Admitted.
 
 Theorem wp_Printf (msg: go_string) (arg: slice.t) :
