new/proof/math.v
@@ -10,6 +10,10 @@ Set Default Proof Using "W".
 #[global] Instance : IsPkgInit (iProp Σ) math := define_is_pkg_init True%I.
 #[global] Instance : GetIsPkgInitWf (iProp Σ) math := build_get_is_pkg_init_wf.
 
+Local Lemma wp_useFMA_init :
+  {{{ True }}} math.useFMA'init #() {{{ RET #(); True }}}.
+Proof. Admitted.
+
 Lemma wp_initialize' get_is_pkg_init :
   get_is_pkg_init_prop math get_is_pkg_init →
   {{{ own_initializing get_is_pkg_init }}}
@@ -17,10 +21,12 @@ Lemma wp_initialize' get_is_pkg_init :
   {{{ RET #(); own_initializing get_is_pkg_init ∗ is_pkg_init math }}}.
 Proof.
   intros Hinit. wp_start as "Hown".
-  wp_apply (wp_package_init with "[$Hown] HΦ").
+  wp_apply (wp_package_init with "[$Hown] HΦ") as "Hown".
   { destruct Hinit as (-> & ?); done. }
-  iIntros "Hown". wp_auto.
-  iEval (rewrite is_pkg_init_unfold /=). iFrame "∗#".
+  do 52 (wp_apply wp_GlobalAlloc as "?").
+  wp_apply wp_useFMA_init.
+  (* remaining: 51 array CompositeLiterals + stores *)
+  all: admit.
 Admitted.
 
 End wps.
