new/proof/strings.v
@@ -12,12 +12,25 @@ Set Default Proof Using "W".
 #[global] Instance : IsPkgInit (iProp Σ) strings := define_is_pkg_init True%I.
 #[global] Instance : GetIsPkgInitWf (iProp Σ) strings := build_get_is_pkg_init_wf.
 
-Lemma wp_asciiSpace_init :
-  {{{ True }}}
-    strings.asciiSpace'init #()
-  {{{ RET #(); True }}}.
-Proof.
-Admitted.
+Local Lemma wp_asciiSpace_init Φ :
+  (∀ v, Φ v) -∗
+  WP exception_do ((do: #()) ;;;
+    let: "$r0" := (let: "$k0" := #(W64 9) in
+    let: "$v1" := #(W8 1) in
+    let: "$k2" := #(W64 10) in
+    let: "$v3" := #(W8 1) in
+    let: "$k4" := #(W64 11) in
+    let: "$v5" := #(W8 1) in
+    let: "$k6" := #(W64 12) in
+    let: "$v7" := #(W8 1) in
+    let: "$k8" := #(W64 13) in
+    let: "$v9" := #(W8 1) in
+    let: "$k10" := #(W64 32) in
+    let: "$v11" := #(W8 1) in
+    CompositeLiteral (go.ArrayType 256 go.uint8) (LiteralValue [KeyedElement (Some (KeyExpression go.int "$k0")) (ElementExpression go.uint8 "$v1"); KeyedElement (Some (KeyExpression go.int "$k2")) (ElementExpression go.uint8 "$v3"); KeyedElement (Some (KeyExpression go.int "$k4")) (ElementExpression go.uint8 "$v5"); KeyedElement (Some (KeyExpression go.int "$k6")) (ElementExpression go.uint8 "$v7"); KeyedElement (Some (KeyExpression go.int "$k8")) (ElementExpression go.uint8 "$v9"); KeyedElement (Some (KeyExpression go.int "$k10")) (ElementExpression go.uint8 "$v11")])) in
+    do:  ((GlobalVarAddr strings.asciiSpace #()) <-[go.ArrayType 256 go.uint8] "$r0"))
+  {{ Φ }}.
+Proof. Admitted.
 
 Lemma wp_initialize' get_is_pkg_init :
   get_is_pkg_init_prop strings get_is_pkg_init →
@@ -26,10 +39,11 @@ Lemma wp_initialize' get_is_pkg_init :
   {{{ RET #(); own_initializing get_is_pkg_init ∗ is_pkg_init strings }}}.
 Proof.
   intros Hinit. wp_start as "Hown".
-  wp_apply (wp_package_init with "[$Hown] HΦ").
+  wp_apply (wp_package_init with "[$Hown] HΦ") as "Hown".
   { destruct Hinit as (-> & ?); done. }
-  iIntros "Hown". wp_auto.
-  wp_apply wp_asciiSpace_init.
+  wp_apply wp_GlobalAlloc as "?" --no-auto.
+  (* asciiSpace array literal - CompositeLiteral semantics can't handle KeyExpression *)
+  iApply wp_asciiSpace_init. iIntros.
   iEval (rewrite is_pkg_init_unfold /=). iFrame "∗#". done.
 Qed.
 
